docs/SecureMessagingDocs/Chapters/KEM/FrodoKEM.lean
@@ -34,23 +34,19 @@ $`\todo`
 :::defTitle "frodo_kem_correctness" "FrodoKEM correctness"
 :::
 
-::::theorem "frodo_kem_correctness" (parent := "frodo_kem") (tags := "gh-260")
+::::theorem "frodo_kem_correctness" (parent := "frodo_kem") (tags := "gh-260") (uses := "frodo_kem_scheme")
 $`\todo`
 
 :::leanPill "missing"
 :::
-
-{usesLabel}`uses` {uses "frodo_kem_scheme"}[]
 ::::
 
 :::defTitle "frodo_kem_security" "FrodoKEM security"
 :::
 
-::::theorem "frodo_kem_security" (parent := "frodo_kem") (tags := "gh-261")
+::::theorem "frodo_kem_security" (parent := "frodo_kem") (tags := "gh-261") (uses := "frodo_kem_scheme")
 $`\todo`
 
 :::leanPill "missing"
 :::
-
-{usesLabel}`uses` {uses "frodo_kem_scheme"}[]
 ::::
