docs/SecureMessagingDocs/Chapters/SecureMessaging/DoubleRatchetSignal.lean
@@ -19,59 +19,49 @@ Double Ratchet SM - Signal.
 :::defTitle "secure_messaging_signal_double_ratchet_spec" "Signal Double Ratchet protocol"
 :::
 
-::::definition "secure_messaging_signal_double_ratchet_spec" (parent := "secure_messaging_signal_protocol_double_ratchet") (tags := "gh-129")
+::::definition "secure_messaging_signal_double_ratchet_spec" (parent := "secure_messaging_signal_protocol_double_ratchet") (tags := "gh-129") (uses := "secure_messaging_abstract_double_ratchet_spec, cka, fs_aead_scheme, prf_prng_scheme")
 $`\todo`
 
 :::leanPill "missing"
 :::
-
-{usesLabel}`uses` {uses "secure_messaging_abstract_double_ratchet_spec"}[] · {uses "cka"}[] · {uses "fs_aead_scheme"}[] · {uses "prf_prng_scheme"}[]
 ::::
 
 :::defTitle "secure_messaging_signal_double_ratchet_correctness" "Signal Double Ratchet correctness"
 :::
 
-::::theorem "secure_messaging_signal_double_ratchet_correctness" (parent := "secure_messaging_signal_protocol_double_ratchet") (tags := "gh-130")
+::::theorem "secure_messaging_signal_double_ratchet_correctness" (parent := "secure_messaging_signal_protocol_double_ratchet") (tags := "gh-130") (uses := "secure_messaging_signal_double_ratchet_spec, secure_messaging_abstract_double_ratchet_correctness")
 $`\todo`
 
 :::leanPill "missing"
 :::
-
-{usesLabel}`uses` {uses "secure_messaging_signal_double_ratchet_spec"}[] · {uses "secure_messaging_abstract_double_ratchet_correctness"}[]
 ::::
 
 :::defTitle "secure_messaging_signal_double_ratchet_authenticity" "Signal Double Ratchet authenticity"
 :::
 
-::::theorem "secure_messaging_signal_double_ratchet_authenticity" (parent := "secure_messaging_signal_protocol_double_ratchet") (tags := "gh-131")
+::::theorem "secure_messaging_signal_double_ratchet_authenticity" (parent := "secure_messaging_signal_protocol_double_ratchet") (tags := "gh-131") (uses := "secure_messaging_signal_double_ratchet_spec, secure_messaging_abstract_double_ratchet_authenticity")
 $`\todo`
 
 :::leanPill "missing"
 :::
-
-{usesLabel}`uses` {uses "secure_messaging_signal_double_ratchet_spec"}[] · {uses "secure_messaging_abstract_double_ratchet_authenticity"}[]
 ::::
 
 :::defTitle "secure_messaging_signal_double_ratchet_privacy" "Signal Double Ratchet privacy"
 :::
 
-::::theorem "secure_messaging_signal_double_ratchet_privacy" (parent := "secure_messaging_signal_protocol_double_ratchet") (tags := "gh-132")
+::::theorem "secure_messaging_signal_double_ratchet_privacy" (parent := "secure_messaging_signal_protocol_double_ratchet") (tags := "gh-132") (uses := "secure_messaging_signal_double_ratchet_spec, secure_messaging_abstract_double_ratchet_privacy")
 $`\todo`
 
 :::leanPill "missing"
 :::
-
-{usesLabel}`uses` {uses "secure_messaging_signal_double_ratchet_spec"}[] · {uses "secure_messaging_abstract_double_ratchet_privacy"}[]
 ::::
 
 :::defTitle "secure_messaging_signal_double_ratchet_security" "Signal Double Ratchet security"
 :::
 
-::::theorem "secure_messaging_signal_double_ratchet_security" (parent := "secure_messaging_signal_protocol_double_ratchet") (tags := "gh-133")
+::::theorem "secure_messaging_signal_double_ratchet_security" (parent := "secure_messaging_signal_protocol_double_ratchet") (tags := "gh-133") (uses := "secure_messaging_signal_double_ratchet_spec, secure_messaging_signal_double_ratchet_correctness, secure_messaging_signal_double_ratchet_authenticity, secure_messaging_signal_double_ratchet_privacy")
 $`\todo`
 
 :::leanPill "missing"
 :::
-
-{usesLabel}`uses` {uses "secure_messaging_signal_double_ratchet_spec"}[] · {uses "secure_messaging_signal_double_ratchet_correctness"}[] · {uses "secure_messaging_signal_double_ratchet_authenticity"}[] · {uses "secure_messaging_signal_double_ratchet_privacy"}[]
 ::::
